examples/mutsum/MutGImp0proof.v
@@ -53,16 +53,6 @@ Section SIMMODSEM.
     rewrite unfold_eval_imp.
     eapply Any.downcast_upcast in _UNWRAPN. des.
     unfold unint in *. destruct v; clarify; ss.
-    imp_steps.
-    des_ifs.
-    - imp_steps.
-    - apply Z.eqb_eq in Heq. clarify.
-    - unfold ccall.
-      imp_steps.
-      gstep. econs; ss. i. des; subst. exists 100.
-      imp_steps.
-      Local Transparent vadd.
-      destruct v; ss; clarify; imp_steps.
-  Qed.
+  Admitted.
 
 End SIMMODSEM.
