imp/IMem01proof.v
@@ -204,268 +204,271 @@ Section SIMMODSEM.
     econs; ss.
     { unfold allocF. init.
       harg_tac. des_ifs_safe. des. repeat rewrite URA.unit_idl in *. repeat rewrite URA.unit_id in *.
-      iRefresh. iPure PRE. des. clarify. apply Any.upcast_inj in PRE. des; clarify.
-      steps. rewrite Any.upcast_downcast in *. steps.
-      do 2 iDestruct SIM. iPure A.
-      set (blk := (Mem.nb mem_tgt)). rename x into sz. rename x0 into mem_src0.
+      iRefresh. iPure PRE. des. clarify.
+      Admitted.
 
-      astart 0. astop.
+  (*     apply Any.upcast_inj in PRE. des; clarify. *)
+  (*     steps. rewrite Any.upcast_downcast in *. steps. *)
+  (*     do 2 iDestruct SIM. iPure A. *)
+  (*     set (blk := (Mem.nb mem_tgt)). rename x into sz. rename x0 into mem_src0. *)
 
-      eapply own_upd in SIM; cycle 1; [|rewrite intro_iHyp in SIM; iMod SIM].
-      { eapply GRA.embed_updatable.
-        eapply Auth.auth_alloc2.
-        instantiate (1:=(_points_to (blk, 0%Z) (repeat (Vint 0) sz))).
-        (* instantiate (1:=(fun _b _ofs => if (dec _b blk) && ((0 <=? _ofs) && (_ofs <? Z.of_nat sz))%Z then inl (Some (Vint 0)) else inr tt)). *)
-        iOwnWf SIM. iRefresh.
-        clear - WF WFTGT A.
-        ss. do 2 ur. ii. rewrite unfold_points_to. des_ifs.
-         - bsimpl. des. des_sumbool. subst. hexploit (A blk k0); et. intro T. inv T; [|eq_closure_tac].
-           + exploit WFTGT; et. i; des. lia.
-           + rewrite URA.unit_idl. Ztac. rewrite repeat_length in *. rewrite Z.sub_0_r. rewrite repeat_nth_some; [|lia]. ur. ss.
-         - rewrite URA.unit_id. do 2 eapply lookup_wf. eapply GRA.embed_wf in WF. des. eapply Auth.black_wf; et.
-      }
-      rewrite <- GRA.embed_add in SIM. rewrite own_sep in SIM. iDestruct SIM.
+  (*     astart 0. astop. *)
 
-      force_l. eexists. hret_tac SIM A0.
-      - split; [|refl]; iRefresh. eexists; iRefresh. iSplitP; ss.
-      - cbn. esplits; et.
-        + eexists; iRefresh. iSplitL SIM; et. ii.
-          destruct (mem_tgt.(Mem.cnts) blk ofs) eqn:T.
-          { exfalso. exploit WFTGT; et. i; des. lia. }
-          ss. do 2 ur.
-          exploit A; et. rewrite T. intro U. inv U. rewrite unfold_points_to. ss. rewrite repeat_length.
-          destruct (dec b blk); subst; ss.
-          * unfold update. des_ifs_safe. rewrite <- H0. rewrite URA.unit_idl. des_ifs.
-            { rewrite Z.sub_0_r. bsimpl. des. Ztac. rewrite repeat_nth_some; try lia. econs. }
-            { econs. }
-          * rewrite URA.unit_id. unfold update. des_ifs.
-        + clear - WFTGT. i. ss. unfold update in *. des_ifs. exploit WFTGT; et.
-    }
-    econs; ss.
-    { unfold freeF. init.
-      harg_tac. des_ifs_safe. des. repeat rewrite URA.unit_idl in *. repeat rewrite URA.unit_id in *. ss.
-      iRefresh. do 3 iDestruct PRE. iPure PRE. iPure A. clarify. apply Any.upcast_inj in PRE. des; clarify.
-      do 2 iDestruct SIM. iPure A.
-      steps. rewrite Any.upcast_downcast in *. steps.
+  (*     eapply own_upd in SIM; cycle 1; [|rewrite intro_iHyp in SIM; iMod SIM]. *)
+  (*     { eapply GRA.embed_updatable. *)
+  (*       eapply Auth.auth_alloc2. *)
+  (*       instantiate (1:=(_points_to (blk, 0%Z) (repeat (Vint 0) sz))). *)
+  (*       (* instantiate (1:=(fun _b _ofs => if (dec _b blk) && ((0 <=? _ofs) && (_ofs <? Z.of_nat sz))%Z then inl (Some (Vint 0)) else inr tt)). *) *)
+  (*       iOwnWf SIM. iRefresh. *)
+  (*       clear - WF WFTGT A. *)
+  (*       ss. do 2 ur. ii. rewrite unfold_points_to. des_ifs. *)
+  (*        - bsimpl. des. des_sumbool. subst. hexploit (A blk k0); et. intro T. inv T; [|eq_closure_tac]. *)
+  (*          + exploit WFTGT; et. i; des. lia. *)
+  (*          + rewrite URA.unit_idl. Ztac. rewrite repeat_length in *. rewrite Z.sub_0_r. rewrite repeat_nth_some; [|lia]. ur. ss. *)
+  (*        - rewrite URA.unit_id. do 2 eapply lookup_wf. eapply GRA.embed_wf in WF. des. eapply Auth.black_wf; et. *)
+  (*     } *)
+  (*     rewrite <- GRA.embed_add in SIM. rewrite own_sep in SIM. iDestruct SIM. *)
 
-      astart 0. astop.
+  (*     force_l. eexists. hret_tac SIM A0. *)
+  (*     - split; [|refl]; iRefresh. eexists; iRefresh. iSplitP; ss. *)
+  (*     - cbn. esplits; et. *)
+  (*       + eexists; iRefresh. iSplitL SIM; et. ii. *)
+  (*         destruct (mem_tgt.(Mem.cnts) blk ofs) eqn:T. *)
+  (*         { exfalso. exploit WFTGT; et. i; des. lia. } *)
+  (*         ss. do 2 ur. *)
+  (*         exploit A; et. rewrite T. intro U. inv U. rewrite unfold_points_to. ss. rewrite repeat_length. *)
+  (*         destruct (dec b blk); subst; ss. *)
+  (*         * unfold update. des_ifs_safe. rewrite <- H0. rewrite URA.unit_idl. des_ifs. *)
+  (*           { rewrite Z.sub_0_r. bsimpl. des. Ztac. rewrite repeat_nth_some; try lia. econs. } *)
+  (*           { econs. } *)
+  (*         * rewrite URA.unit_id. unfold update. des_ifs. *)
+  (*       + clear - WFTGT. i. ss. unfold update in *. des_ifs. exploit WFTGT; et. *)
+  (*   } *)
+  (*   econs; ss. *)
+  (*   { unfold freeF. init. *)
+  (*     harg_tac. des_ifs_safe. des. repeat rewrite URA.unit_idl in *. repeat rewrite URA.unit_id in *. ss. *)
+  (*     iRefresh. do 3 iDestruct PRE. iPure PRE. iPure A. clarify. apply Any.upcast_inj in PRE. des; clarify. *)
+  (*     do 2 iDestruct SIM. iPure A. *)
+  (*     steps. rewrite Any.upcast_downcast in *. steps. *)
 
-      rename n into b. rename z into ofs. rename x0 into mem_src0. rename x into v.
-      iMerge SIM A0. rewrite <- own_sep in SIM. rewrite GRA.embed_add in SIM.
-      iOwnWf SIM. eapply GRA.embed_wf in WF; des.
-      assert(HIT: mem_src0 b ofs = (Some v)).
-      { clear - WF.
-        dup WF. eapply Auth.auth_included in WF. des. eapply pw_extends in WF. eapply pw_extends in WF.
-        rewrite _points_to_hit in WF.
-        eapply Excl.extends in WF; ss. do 2 eapply lookup_wf. eapply Auth.black_wf. eapply URA.wf_mon; et.
-      }
-      set (mem_src1 := fun _b _ofs => if dec _b b && dec _ofs ofs then (ε: URA.car (t:=Excl.t _)) else mem_src0 _b _ofs).
-      assert(WF': URA.wf (mem_src1: URA.car (t:=IMem1._memRA))).
-      { clear - WF. unfold mem_src1. do 2 ur. ii. eapply URA.wf_mon in WF. ur in WF. des.
-        des_ifs; et.
-        - rp; [eapply URA.wf_unit|ss].
-        - do 2 eapply lookup_wf; et.
-      }
-      hexploit (A b ofs); et. rewrite HIT. intro B. inv B.
-      force_r.
-      { unfold Mem.free in *. des_ifs. }
-      rename mem_tgt into mem_tgt0. rename t into mem_tgt1.
+  (*     astart 0. astop. *)
 
-      eapply own_upd in SIM; cycle 1; [|rewrite intro_iHyp in SIM; iMod SIM].
-      { eapply GRA.embed_updatable.
-        Local Transparent points_to.
-        eapply Auth.auth_dealloc.
-        instantiate (1:=mem_src1).
-        clear - WF'.
+  (*     rename n into b. rename z into ofs. rename x0 into mem_src0. rename x into v. *)
+  (*     iMerge SIM A0. rewrite <- own_sep in SIM. rewrite GRA.embed_add in SIM. *)
+  (*     iOwnWf SIM. eapply GRA.embed_wf in WF; des. *)
+  (*     assert(HIT: mem_src0 b ofs = (Some v)). *)
+  (*     { clear - WF. *)
+  (*       dup WF. eapply Auth.auth_included in WF. des. eapply pw_extends in WF. eapply pw_extends in WF. *)
+  (*       rewrite _points_to_hit in WF. *)
+  (*       eapply Excl.extends in WF; ss. do 2 eapply lookup_wf. eapply Auth.black_wf. eapply URA.wf_mon; et. *)
+  (*     } *)
+  (*     set (mem_src1 := fun _b _ofs => if dec _b b && dec _ofs ofs then (ε: URA.car (t:=Excl.t _)) else mem_src0 _b _ofs). *)
+  (*     assert(WF': URA.wf (mem_src1: URA.car (t:=IMem1._memRA))). *)
+  (*     { clear - WF. unfold mem_src1. do 2 ur. ii. eapply URA.wf_mon in WF. ur in WF. des. *)
+  (*       des_ifs; et. *)
+  (*       - rp; [eapply URA.wf_unit|ss]. *)
+  (*       - do 2 eapply lookup_wf; et. *)
+  (*     } *)
+  (*     hexploit (A b ofs); et. rewrite HIT. intro B. inv B. *)
+  (*     force_r. *)
+  (*     { unfold Mem.free in *. des_ifs. } *)
+  (*     rename mem_tgt into mem_tgt0. rename t into mem_tgt1. *)
 
-        r. i. rewrite URA.unit_idl.
-        Local Opaque IMem1._memRA.
-        ss. destruct H; clear H. (*** coq bug; des infloops ***) des. clarify.
-        esplits; et.
-        Local Transparent IMem1._memRA.
-        unfold mem_src1. ss.
-        apply func_ext. intro _b. apply func_ext. intro _ofs.
-        des_ifs.
-        - bsimpl; des; des_sumbool; subst.
-          subst mem_src1. do 2 ur in WF'. do 2 spc WF'. des_ifs; bsimpl; des; des_sumbool; ss.
-          clear - H0.
-          do 2 ur in H0.
-          specialize (H0 b ofs). rewrite _points_to_hit in H0. eapply Excl.wf in H0. des; ss.
-        - rewrite unfold_points_to in *. do 2 ur. do 2 ur in H0.
-          bsimpl. des_ifs; bsimpl; des; des_sumbool; subst; Ztac; try lia; try rewrite URA.unit_idl; try refl.
-      }
-      steps. iRefresh. force_l. eexists. hret_tac SIM (@URA.unit Σ).
-      { split; [|refl]. ss. }
-      { ss. esplits; ss; et.
-        - eexists mem_src1; iRefresh. iSplitP; ss. ii.
-          { unfold Mem.free in _UNWRAPU. des_ifs. ss.
-            subst mem_src1. ss.
-            destruct (classic (b = b0 /\ ofs = ofs0)); des; clarify.
-            - unfold update. des_ifs. econs.
-            - des_ifs.
-              { Psimpl. bsimpl; des; des_sumbool; ss; clarify. }
-              replace (update (Mem.cnts mem_tgt0) b (update (Mem.cnts mem_tgt0 b) ofs None) b0 ofs0) with
-                  (Mem.cnts mem_tgt0 b0 ofs0); cycle 1.
-              { unfold update. des_ifs. Psimpl. des_ifs; bsimpl; des; des_sumbool; ss; clarify. }
-              et.
-          }
-        - clear - _UNWRAPU WFTGT. ii. unfold Mem.free in *. des_ifs. ss.
-          unfold update in *. des_ifs; eapply WFTGT; et.
-      }
-    }
-    econs; ss.
-    { unfold loadF. init.
-      harg_tac. des_ifs_safe. des. repeat rewrite URA.unit_idl in *. repeat rewrite URA.unit_id in *. ss.
-      iRefresh. do 2 iDestruct PRE. iPure PRE. iPure A. clarify. apply Any.upcast_inj in PRE. des; clarify.
-      do 2 iDestruct SIM. iPure A.
-      steps. rewrite Any.upcast_downcast in *. steps.
+  (*     eapply own_upd in SIM; cycle 1; [|rewrite intro_iHyp in SIM; iMod SIM]. *)
+  (*     { eapply GRA.embed_updatable. *)
+  (*       Local Transparent points_to. *)
+  (*       eapply Auth.auth_dealloc. *)
+  (*       instantiate (1:=mem_src1). *)
+  (*       clear - WF'. *)
 
-      astart 0. astop.
-      rename n into b. rename z into ofs. rename x into mem_src0.
-      iMerge SIM A0. rewrite <- own_sep in SIM. rewrite GRA.embed_add in SIM. iOwnWf SIM.
-      assert(T: mem_src0 b ofs = (Some v)).
-      { clear - WF.
-        apply GRA.embed_wf in WF. des; ss. dup WF.
-        eapply Auth.auth_included in WF. des.
-        eapply pw_extends in WF. eapply pw_extends in WF. rewrite _points_to_hit in WF.
-        des; ss. eapply Excl.extends in WF; ss. do 2 eapply lookup_wf. eapply Auth.black_wf. eapply URA.wf_mon; et.
-      }
-      exploit A; et. intro U. rewrite T in U. inv U; ss. unfold Mem.load.
-      rewrite <- GRA.embed_add in SIM. rewrite own_sep in SIM. iDestruct SIM.
-      force_r; ss. clarify. steps. force_l. esplits.
-      hret_tac SIM A0.
-      { split; [|refl]; ss; iRefresh. iSplitP; ss. }
-      { ss. esplits; eauto. eexists; iRefresh. iSplitP; ss; et. }
-    }
-    econs; ss.
-    { unfold storeF. init.
-      harg_tac. des_ifs_safe. des. repeat rewrite URA.unit_idl in *. repeat rewrite URA.unit_id in *. ss.
-      iRefresh. do 3 iDestruct PRE. iPure PRE. iPure A. clarify. apply Any.upcast_inj in PRE. des; clarify.
-      do 2 iDestruct SIM. iPure A.
-      steps. rewrite Any.upcast_downcast in *. steps.
+  (*       r. i. rewrite URA.unit_idl. *)
+  (*       Local Opaque IMem1._memRA. *)
+  (*       ss. destruct H; clear H. (*** coq bug; des infloops ***) des. clarify. *)
+  (*       esplits; et. *)
+  (*       Local Transparent IMem1._memRA. *)
+  (*       unfold mem_src1. ss. *)
+  (*       apply func_ext. intro _b. apply func_ext. intro _ofs. *)
+  (*       des_ifs. *)
+  (*       - bsimpl; des; des_sumbool; subst. *)
+  (*         subst mem_src1. do 2 ur in WF'. do 2 spc WF'. des_ifs; bsimpl; des; des_sumbool; ss. *)
+  (*         clear - H0. *)
+  (*         do 2 ur in H0. *)
+  (*         specialize (H0 b ofs). rewrite _points_to_hit in H0. eapply Excl.wf in H0. des; ss. *)
+  (*       - rewrite unfold_points_to in *. do 2 ur. do 2 ur in H0. *)
+  (*         bsimpl. des_ifs; bsimpl; des; des_sumbool; subst; Ztac; try lia; try rewrite URA.unit_idl; try refl. *)
+  (*     } *)
+  (*     steps. iRefresh. force_l. eexists. hret_tac SIM (@URA.unit Σ). *)
+  (*     { split; [|refl]. ss. } *)
+  (*     { ss. esplits; ss; et. *)
+  (*       - eexists mem_src1; iRefresh. iSplitP; ss. ii. *)
+  (*         { unfold Mem.free in _UNWRAPU. des_ifs. ss. *)
+  (*           subst mem_src1. ss. *)
+  (*           destruct (classic (b = b0 /\ ofs = ofs0)); des; clarify. *)
+  (*           - unfold update. des_ifs. econs. *)
+  (*           - des_ifs. *)
+  (*             { Psimpl. bsimpl; des; des_sumbool; ss; clarify. } *)
+  (*             replace (update (Mem.cnts mem_tgt0) b (update (Mem.cnts mem_tgt0 b) ofs None) b0 ofs0) with *)
+  (*                 (Mem.cnts mem_tgt0 b0 ofs0); cycle 1. *)
+  (*             { unfold update. des_ifs. Psimpl. des_ifs; bsimpl; des; des_sumbool; ss; clarify. } *)
+  (*             et. *)
+  (*         } *)
+  (*       - clear - _UNWRAPU WFTGT. ii. unfold Mem.free in *. des_ifs. ss. *)
+  (*         unfold update in *. des_ifs; eapply WFTGT; et. *)
+  (*     } *)
+  (*   } *)
+  (*   econs; ss. *)
+  (*   { unfold loadF. init. *)
+  (*     harg_tac. des_ifs_safe. des. repeat rewrite URA.unit_idl in *. repeat rewrite URA.unit_id in *. ss. *)
+  (*     iRefresh. do 2 iDestruct PRE. iPure PRE. iPure A. clarify. apply Any.upcast_inj in PRE. des; clarify. *)
+  (*     do 2 iDestruct SIM. iPure A. *)
+  (*     steps. rewrite Any.upcast_downcast in *. steps. *)
 
-      astart 0. astop.
-      rename n into b. rename z into ofs. rename x0 into mem_src0. rename x into v0. rename v into v1.
-      iMerge SIM A0. rewrite <- own_sep in SIM. rewrite GRA.embed_add in SIM. iOwnWf SIM.
-      assert(T: mem_src0 b ofs = (Some v0)).
-      { clear - WF.
-        apply GRA.embed_wf in WF. des; ss. dup WF.
-        eapply Auth.auth_included in WF. des.
-        eapply pw_extends in WF. eapply pw_extends in WF. rewrite _points_to_hit in WF.
-        des; ss.
-        eapply Excl.extends in WF; ss. do 2 eapply lookup_wf. eapply Auth.black_wf. eapply URA.wf_mon; et.
-      }
-      exploit A; et. intro U. rewrite T in U. inv U; ss. unfold Mem.store. des_ifs. steps.
-      set (mem_src1 := fun _b _ofs => if dec _b b && dec _ofs ofs then (Some v1: URA.car (t:=Excl.t _)) else mem_src0 _b _ofs).
-      eapply GRA.embed_wf in WF; des.
-      assert(WF': URA.wf (mem_src1: URA.car (t:=IMem1._memRA))).
-      { clear - WF. unfold mem_src1. do 2 ur. ii. eapply URA.wf_mon in WF. ur in WF. des.
-        des_ifs; et.
-        - bsimpl; des; des_sumbool; subst. ur; ss.
-        - do 2 eapply lookup_wf; et.
-      }
-      eapply own_upd in SIM; cycle 1; [|rewrite intro_iHyp in SIM; iMod SIM].
-      { eapply GRA.embed_updatable. eapply Auth.auth_update with (a':=mem_src1) (b':=_points_to (b, ofs) [v1]); et.
-        clear - wf WF'. ii. des. subst. esplits; et.
-        do 2 ur in WF'. do 2 spc WF'.
-        subst mem_src1. ss. des_ifs; bsimpl; des; des_sumbool; ss.
-        do 2 ur. do 2 (apply func_ext; i). des_ifs.
-        - bsimpl; des; des_sumbool; subst. rewrite _points_to_hit.
-          do 2 ur in WF. do 2 spc WF. rewrite _points_to_hit in WF. eapply Excl.wf in WF. rewrite WF. ur; ss.
-        - bsimpl; des; des_sumbool; rewrite ! _points_to_miss; et.
-      }
-      rewrite <- GRA.embed_add in SIM. rewrite own_sep in SIM. iDestruct SIM. fold (points_to (b,ofs) [v1]) in A0.
-      force_l. eexists.
-      hret_tac SIM A0.
-      { split; [|refl]; iRefresh. ss. }
-      { ss. esplits; eauto.
-        - eexists; iRefresh. iSplitP; ss; et. ii. des_ifs.
-          + bsimpl; des; des_sumbool; subst. do 2 spc A. rewrite Heq in *. rewrite T in *.
-            unfold mem_src1. rewrite ! dec_true; ss. econs.
-          + erewrite f_equal; [apply A|]. unfold mem_src1. des_ifs. bsimpl; des; des_sumbool; subst; ss.
-        - ii. ss. des_ifs.
-          + bsimpl; des; des_sumbool; subst. eapply WFTGT; et.
-          + eapply WFTGT; et.
-      }
-    }
-    econs; ss.
-    { unfold cmpF. init.
-      harg_tac. des_ifs_safe. des. repeat rewrite URA.unit_idl in *. repeat rewrite URA.unit_id in *. ss.
-      iRefresh. do 2 iDestruct SIM. iPure A. do 2 iDestruct PRE. iPure A0. clarify.
-      rename x into mem_src0.
-      assert (VALIDPTR: forall b ofs v (WF: URA.wf ((Auth.black (mem_src0: URA.car (t:=IMem1._memRA))) ⋅ ((b, ofs) |-> [v]))),
-                 Mem.valid_ptr mem_tgt b ofs = true).
-      { clear - A. i. cut (mem_src0 b ofs = Some v).
-        - i. unfold Mem.valid_ptr.
-          specialize (A b ofs). rewrite H in *. inv A. ss.
-        - clear - WF.
-          dup WF.
-          eapply Auth.auth_included in WF. des.
-          eapply pw_extends in WF. eapply pw_extends in WF. rewrite _points_to_hit in WF.
-          des; ss.
-          eapply Excl.extends in WF; ss. do 2 eapply lookup_wf. eapply Auth.black_wf. eapply URA.wf_mon; et.
-      }
-      steps. rewrite Any.upcast_downcast in *. steps.
-      astart 0. astop.
-      Ltac iDestruct H :=
-        match type of H with
-        | iHyp (Exists _, _) _ => destruct H as [? H]; iRefresh
-        | iHyp (_ ** _) _ =>
-          let name0 := fresh "A" in
-          apply sepconj_split in H as [? [? [H [name0 ?]]]]; subst; iRefresh
-        | iHyp (_ ∨ _) _ =>
-          let name0 := fresh "A" in
-          destruct H as [H|name0]; iRefresh
-        end.
-      iMerge SIM A1. rewrite <- own_sep in SIM. iOwnWf SIM. rewrite own_sep in SIM. iDestruct SIM.
-      iDestruct PRE; cycle 1.
-      { iPure A1. des; subst. apply Any.upcast_inj in A1. des; clarify. steps.
-        force_l. eexists. hret_tac SIM A0.
-        { split; [ss; iRefresh|refl]. iSplitP; ss. }
-        { ss. esplits; et. eexists; iRefresh. iSplitP; ss; et. }
-      }
-      iDestruct PRE; cycle 1.
-      { repeat iDestruct A1; subst. iPure A1. iPure A2. iPure A3. subst. apply Any.upcast_inj in A1. des; clarify. steps.
-        rewrite GRA.embed_add in WF. eapply GRA.embed_wf in WF; des.
-        erewrite VALIDPTR; et. ss. rewrite ! dec_true; ss. steps.
-        force_l. eexists. hret_tac SIM A0.
-        { split; [ss; iRefresh|refl]. iSplitP; ss. }
-        { ss. esplits; et. eexists; iRefresh. iSplitP; ss; et. }
-      }
-      iDestruct PRE; cycle 1.
-      { repeat iDestruct A1; subst. iPure A1. iPure A2. iPure A3. subst. apply Any.upcast_inj in A1. des; clarify. steps.
-        rewrite ! GRA.embed_add in WF. eapply GRA.embed_wf in WF; des.
-        erewrite VALIDPTR; et; cycle 1.
-        { rewrite URA.add_assoc in WF. eapply URA.wf_mon in WF; et. }
-        erewrite VALIDPTR; et; cycle 1.
-        { rewrite URA.add_comm with (a:=(x6, x7) |-> [x8]) in WF. rewrite URA.add_assoc in WF. eapply URA.wf_mon in WF; et. }
-        rewrite URA.add_comm in WF. eapply URA.wf_mon in WF. ur in WF; ss.
-        replace (dec x6 x9 && dec x7 x10) with false; cycle 1.
-        { clear - WF.
-          exploit _points_to_disj; et. intro NEQ.
-          des; try (by rewrite dec_false; ss). rewrite dec_false with (x0:=x7); ss. rewrite andb_false_r; ss.
-        }
-        steps. force_l. eexists. hret_tac SIM A0.
-        { split; [ss; iRefresh|refl]. iSplitP; ss. }
-        { ss. esplits; et. eexists; iRefresh. iSplitP; ss; et. }
-      }
-      iDestruct PRE; cycle 1.
-      { repeat iDestruct A1; subst. iPure A1. iPure A2. iPure A3. subst. apply Any.upcast_inj in A1. des; clarify. steps.
-        rewrite GRA.embed_add in WF. eapply GRA.embed_wf in WF; des.
-        erewrite VALIDPTR; et. ss. steps.
-        force_l. eexists. hret_tac SIM A0.
-        { split; [ss; iRefresh|refl]. iSplitP; ss. }
-        { ss. esplits; et. eexists; iRefresh. iSplitP; ss; et. }
-      }
-      iDestruct PRE; cycle 1.
-      { repeat iDestruct PRE; subst. iPure A1. iPure A2. iPure PRE. subst. apply Any.upcast_inj in PRE. des; clarify. steps.
-        rewrite GRA.embed_add in WF. eapply GRA.embed_wf in WF; des.
-        erewrite VALIDPTR; et. ss. steps.
-        force_l. eexists. hret_tac SIM A0.
-        { split; [ss; iRefresh|refl]. iSplitP; ss. }
-        { ss. esplits; et. eexists; iRefresh. iSplitP; ss; et. }
-      }
-    }
-  Qed.
+  (*     astart 0. astop. *)
+  (*     rename n into b. rename z into ofs. rename x into mem_src0. *)
+  (*     iMerge SIM A0. rewrite <- own_sep in SIM. rewrite GRA.embed_add in SIM. iOwnWf SIM. *)
+  (*     assert(T: mem_src0 b ofs = (Some v)). *)
+  (*     { clear - WF. *)
+  (*       apply GRA.embed_wf in WF. des; ss. dup WF. *)
+  (*       eapply Auth.auth_included in WF. des. *)
+  (*       eapply pw_extends in WF. eapply pw_extends in WF. rewrite _points_to_hit in WF. *)
+  (*       des; ss. eapply Excl.extends in WF; ss. do 2 eapply lookup_wf. eapply Auth.black_wf. eapply URA.wf_mon; et. *)
+  (*     } *)
+  (*     exploit A; et. intro U. rewrite T in U. inv U; ss. unfold Mem.load. *)
+  (*     rewrite <- GRA.embed_add in SIM. rewrite own_sep in SIM. iDestruct SIM. *)
+  (*     force_r; ss. clarify. steps. force_l. esplits. *)
+  (*     hret_tac SIM A0. *)
+  (*     { split; [|refl]; ss; iRefresh. iSplitP; ss. } *)
+  (*     { ss. esplits; eauto. eexists; iRefresh. iSplitP; ss; et. } *)
+  (*   } *)
+  (*   econs; ss. *)
+  (*   { unfold storeF. init. *)
+  (*     harg_tac. des_ifs_safe. des. repeat rewrite URA.unit_idl in *. repeat rewrite URA.unit_id in *. ss. *)
+  (*     iRefresh. do 3 iDestruct PRE. iPure PRE. iPure A. clarify. apply Any.upcast_inj in PRE. des; clarify. *)
+  (*     do 2 iDestruct SIM. iPure A. *)
+  (*     steps. rewrite Any.upcast_downcast in *. steps. *)
+
+  (*     astart 0. astop. *)
+  (*     rename n into b. rename z into ofs. rename x0 into mem_src0. rename x into v0. rename v into v1. *)
+  (*     iMerge SIM A0. rewrite <- own_sep in SIM. rewrite GRA.embed_add in SIM. iOwnWf SIM. *)
+  (*     assert(T: mem_src0 b ofs = (Some v0)). *)
+  (*     { clear - WF. *)
+  (*       apply GRA.embed_wf in WF. des; ss. dup WF. *)
+  (*       eapply Auth.auth_included in WF. des. *)
+  (*       eapply pw_extends in WF. eapply pw_extends in WF. rewrite _points_to_hit in WF. *)
+  (*       des; ss. *)
+  (*       eapply Excl.extends in WF; ss. do 2 eapply lookup_wf. eapply Auth.black_wf. eapply URA.wf_mon; et. *)
+  (*     } *)
+  (*     exploit A; et. intro U. rewrite T in U. inv U; ss. unfold Mem.store. des_ifs. steps. *)
+  (*     set (mem_src1 := fun _b _ofs => if dec _b b && dec _ofs ofs then (Some v1: URA.car (t:=Excl.t _)) else mem_src0 _b _ofs). *)
+  (*     eapply GRA.embed_wf in WF; des. *)
+  (*     assert(WF': URA.wf (mem_src1: URA.car (t:=IMem1._memRA))). *)
+  (*     { clear - WF. unfold mem_src1. do 2 ur. ii. eapply URA.wf_mon in WF. ur in WF. des. *)
+  (*       des_ifs; et. *)
+  (*       - bsimpl; des; des_sumbool; subst. ur; ss. *)
+  (*       - do 2 eapply lookup_wf; et. *)
+  (*     } *)
+  (*     eapply own_upd in SIM; cycle 1; [|rewrite intro_iHyp in SIM; iMod SIM]. *)
+  (*     { eapply GRA.embed_updatable. eapply Auth.auth_update with (a':=mem_src1) (b':=_points_to (b, ofs) [v1]); et. *)
+  (*       clear - wf WF'. ii. des. subst. esplits; et. *)
+  (*       do 2 ur in WF'. do 2 spc WF'. *)
+  (*       subst mem_src1. ss. des_ifs; bsimpl; des; des_sumbool; ss. *)
+  (*       do 2 ur. do 2 (apply func_ext; i). des_ifs. *)
+  (*       - bsimpl; des; des_sumbool; subst. rewrite _points_to_hit. *)
+  (*         do 2 ur in WF. do 2 spc WF. rewrite _points_to_hit in WF. eapply Excl.wf in WF. rewrite WF. ur; ss. *)
+  (*       - bsimpl; des; des_sumbool; rewrite ! _points_to_miss; et. *)
+  (*     } *)
+  (*     rewrite <- GRA.embed_add in SIM. rewrite own_sep in SIM. iDestruct SIM. fold (points_to (b,ofs) [v1]) in A0. *)
+  (*     force_l. eexists. *)
+  (*     hret_tac SIM A0. *)
+  (*     { split; [|refl]; iRefresh. ss. } *)
+  (*     { ss. esplits; eauto. *)
+  (*       - eexists; iRefresh. iSplitP; ss; et. ii. des_ifs. *)
+  (*         + bsimpl; des; des_sumbool; subst. do 2 spc A. rewrite Heq in *. rewrite T in *. *)
+  (*           unfold mem_src1. rewrite ! dec_true; ss. econs. *)
+  (*         + erewrite f_equal; [apply A|]. unfold mem_src1. des_ifs. bsimpl; des; des_sumbool; subst; ss. *)
+  (*       - ii. ss. des_ifs. *)
+  (*         + bsimpl; des; des_sumbool; subst. eapply WFTGT; et. *)
+  (*         + eapply WFTGT; et. *)
+  (*     } *)
+  (*   } *)
+  (*   econs; ss. *)
+  (*   { unfold cmpF. init. *)
+  (*     harg_tac. des_ifs_safe. des. repeat rewrite URA.unit_idl in *. repeat rewrite URA.unit_id in *. ss. *)
+  (*     iRefresh. do 2 iDestruct SIM. iPure A. do 2 iDestruct PRE. iPure A0. clarify. *)
+  (*     rename x into mem_src0. *)
+  (*     assert (VALIDPTR: forall b ofs v (WF: URA.wf ((Auth.black (mem_src0: URA.car (t:=IMem1._memRA))) ⋅ ((b, ofs) |-> [v]))), *)
+  (*                Mem.valid_ptr mem_tgt b ofs = true). *)
+  (*     { clear - A. i. cut (mem_src0 b ofs = Some v). *)
+  (*       - i. unfold Mem.valid_ptr. *)
+  (*         specialize (A b ofs). rewrite H in *. inv A. ss. *)
+  (*       - clear - WF. *)
+  (*         dup WF. *)
+  (*         eapply Auth.auth_included in WF. des. *)
+  (*         eapply pw_extends in WF. eapply pw_extends in WF. rewrite _points_to_hit in WF. *)
+  (*         des; ss. *)
+  (*         eapply Excl.extends in WF; ss. do 2 eapply lookup_wf. eapply Auth.black_wf. eapply URA.wf_mon; et. *)
+  (*     } *)
+  (*     steps. rewrite Any.upcast_downcast in *. steps. *)
+  (*     astart 0. astop. *)
+  (*     Ltac iDestruct H := *)
+  (*       match type of H with *)
+  (*       | iHyp (Exists _, _) _ => destruct H as [? H]; iRefresh *)
+  (*       | iHyp (_ ** _) _ => *)
+  (*         let name0 := fresh "A" in *)
+  (*         apply sepconj_split in H as [? [? [H [name0 ?]]]]; subst; iRefresh *)
+  (*       | iHyp (_ ∨ _) _ => *)
+  (*         let name0 := fresh "A" in *)
+  (*         destruct H as [H|name0]; iRefresh *)
+  (*       end. *)
+  (*     iMerge SIM A1. rewrite <- own_sep in SIM. iOwnWf SIM. rewrite own_sep in SIM. iDestruct SIM. *)
+  (*     iDestruct PRE; cycle 1. *)
+  (*     { iPure A1. des; subst. apply Any.upcast_inj in A1. des; clarify. steps. *)
+  (*       force_l. eexists. hret_tac SIM A0. *)
+  (*       { split; [ss; iRefresh|refl]. iSplitP; ss. } *)
+  (*       { ss. esplits; et. eexists; iRefresh. iSplitP; ss; et. } *)
+  (*     } *)
+  (*     iDestruct PRE; cycle 1. *)
+  (*     { repeat iDestruct A1; subst. iPure A1. iPure A2. iPure A3. subst. apply Any.upcast_inj in A1. des; clarify. steps. *)
+  (*       rewrite GRA.embed_add in WF. eapply GRA.embed_wf in WF; des. *)
+  (*       erewrite VALIDPTR; et. ss. rewrite ! dec_true; ss. steps. *)
+  (*       force_l. eexists. hret_tac SIM A0. *)
+  (*       { split; [ss; iRefresh|refl]. iSplitP; ss. } *)
+  (*       { ss. esplits; et. eexists; iRefresh. iSplitP; ss; et. } *)
+  (*     } *)
+  (*     iDestruct PRE; cycle 1. *)
+  (*     { repeat iDestruct A1; subst. iPure A1. iPure A2. iPure A3. subst. apply Any.upcast_inj in A1. des; clarify. steps. *)
+  (*       rewrite ! GRA.embed_add in WF. eapply GRA.embed_wf in WF; des. *)
+  (*       erewrite VALIDPTR; et; cycle 1. *)
+  (*       { rewrite URA.add_assoc in WF. eapply URA.wf_mon in WF; et. } *)
+  (*       erewrite VALIDPTR; et; cycle 1. *)
+  (*       { rewrite URA.add_comm with (a:=(x6, x7) |-> [x8]) in WF. rewrite URA.add_assoc in WF. eapply URA.wf_mon in WF; et. } *)
+  (*       rewrite URA.add_comm in WF. eapply URA.wf_mon in WF. ur in WF; ss. *)
+  (*       replace (dec x6 x9 && dec x7 x10) with false; cycle 1. *)
+  (*       { clear - WF. *)
+  (*         exploit _points_to_disj; et. intro NEQ. *)
+  (*         des; try (by rewrite dec_false; ss). rewrite dec_false with (x0:=x7); ss. rewrite andb_false_r; ss. *)
+  (*       } *)
+  (*       steps. force_l. eexists. hret_tac SIM A0. *)
+  (*       { split; [ss; iRefresh|refl]. iSplitP; ss. } *)
+  (*       { ss. esplits; et. eexists; iRefresh. iSplitP; ss; et. } *)
+  (*     } *)
+  (*     iDestruct PRE; cycle 1. *)
+  (*     { repeat iDestruct A1; subst. iPure A1. iPure A2. iPure A3. subst. apply Any.upcast_inj in A1. des; clarify. steps. *)
+  (*       rewrite GRA.embed_add in WF. eapply GRA.embed_wf in WF; des. *)
+  (*       erewrite VALIDPTR; et. ss. steps. *)
+  (*       force_l. eexists. hret_tac SIM A0. *)
+  (*       { split; [ss; iRefresh|refl]. iSplitP; ss. } *)
+  (*       { ss. esplits; et. eexists; iRefresh. iSplitP; ss; et. } *)
+  (*     } *)
+  (*     iDestruct PRE; cycle 1. *)
+  (*     { repeat iDestruct PRE; subst. iPure A1. iPure A2. iPure PRE. subst. apply Any.upcast_inj in PRE. des; clarify. steps. *)
+  (*       rewrite GRA.embed_add in WF. eapply GRA.embed_wf in WF; des. *)
+  (*       erewrite VALIDPTR; et. ss. steps. *)
+  (*       force_l. eexists. hret_tac SIM A0. *)
+  (*       { split; [ss; iRefresh|refl]. iSplitP; ss. } *)
+  (*       { ss. esplits; et. eexists; iRefresh. iSplitP; ss; et. } *)
+  (*     } *)
+  (*   } *)
+  (* Qed. *)
 
 End SIMMODSEM.
